Semantic/Consume/Syntax/Exp.lean
@@ -12,13 +12,11 @@ inductive Exp : Sig -> Type where
 | abs : CaptureSet s -> Ty .capt s -> Exp (s,x) -> Exp s
 | tabs : CaptureSet s -> PureTy s -> Exp (s,X) -> Exp s
 | cabs : CaptureSet s -> CaptureBound s -> Exp (s,C) -> Exp s
-| boxed : CaptureSet s -> SepCtx s -> Exp s -> Exp s
 | reader : Var .var s -> Exp s
 | pack : CaptureSet s -> Var .var s -> Exp s
 | app : Var .var s -> Var .var s -> Exp s
 | tapp : Var .var s -> PureTy s -> Exp s
 | capp : Var .var s -> CaptureSet s -> Exp s
-| unwrap : Var .var s -> Exp s
 | letin : Exp s -> Exp (s,x) -> Exp s
 | unpack : Exp s -> Exp ((s,C),x) -> Exp s
 | unit : Exp s
@@ -35,13 +33,11 @@ def Exp.rename : Exp s1 -> Rename s1 s2 -> Exp s2
 | .abs cs T e, f => .abs (cs.rename f) (T.rename f) (e.rename (f.lift))
 | .tabs cs T e, f => .tabs (cs.rename f) (T.rename f) (e.rename (f.lift))
 | .cabs cs cb e, f => .cabs (cs.rename f) (cb.rename f) (e.rename (f.lift))
-| .boxed cs Ψ e, f => .boxed (cs.rename f) (Ψ.rename f) (e.rename f)
 | .reader x, f => .reader (x.rename f)
 | .pack cs x, f => .pack (cs.rename f) (x.rename f)
 | .app x y, f => .app (x.rename f) (y.rename f)
 | .tapp x T, f => .tapp (x.rename f) (T.rename f)
 | .capp x cs, f => .capp (x.rename f) (cs.rename f)
-| .unwrap x, f => .unwrap (x.rename f)
 | .letin e1 e2, f => .letin (e1.rename f) (e2.rename (f.lift))
 | .unpack e1 e2, f => .unpack (e1.rename f) (e2.rename (f.lift.lift))
 | .unit, _ => .unit
@@ -57,7 +53,6 @@ inductive Exp.IsVal : Exp s -> Prop where
 | abs : Exp.IsVal (.abs cs T e)
 | tabs : Exp.IsVal (.tabs cs T e)
 | cabs : Exp.IsVal (.cabs cs m e)
-| boxed : Exp.IsVal (.boxed cs Ψ e)
 | pack : Exp.IsVal (.pack cs x)
 | reader : Exp.IsVal (.reader x)
 | unit : Exp.IsVal .unit
@@ -70,7 +65,6 @@ inductive Exp.IsSimpleVal : Exp s -> Prop where
 | abs : Exp.IsSimpleVal (.abs cs T e)
 | tabs : Exp.IsSimpleVal (.tabs cs T e)
 | cabs : Exp.IsSimpleVal (.cabs cs m e)
-| boxed : Exp.IsSimpleVal (.boxed cs Ψ e)
 | unit : Exp.IsSimpleVal .unit
 | btrue : Exp.IsSimpleVal .btrue
 | bfalse : Exp.IsSimpleVal .bfalse
@@ -100,7 +94,7 @@ def Exp.rename_id {e : Exp s} : e.rename (Rename.id) = e := by
   induction e
   all_goals
     simp [Exp.rename, Ty.rename_id, PureTy.rename_id, Var.rename_id,
-      CaptureSet.rename_id, CaptureBound.rename_id, SepCtx.rename_id, Rename.lift_id, *]
+      CaptureSet.rename_id, CaptureBound.rename_id, Rename.lift_id, *]
 
 /-- Renaming distributes over composition of renamings. -/
 theorem Var.rename_comp {x : Var k s1} {f : Rename s1 s2} {g : Rename s2 s3} :
@@ -113,7 +107,7 @@ theorem Exp.rename_comp {e : Exp s1} {f : Rename s1 s2} {g : Rename s2 s3} :
   induction e generalizing s2 s3
   all_goals
     simp [Exp.rename, Ty.rename_comp, PureTy.rename_comp, Var.rename_comp,
-      CaptureSet.rename_comp, CaptureBound.rename_comp, SepCtx.rename_comp, Rename.lift_comp, *]
+      CaptureSet.rename_comp, CaptureBound.rename_comp, Rename.lift_comp, *]
 
 /-- Weakening commutes with renaming under a binder. -/
 theorem Var.weaken_rename_comm {x : Var k s1} {f : Rename s1 s2} :
@@ -137,14 +131,11 @@ inductive Exp.IsClosed : Exp s -> Prop where
     Exp.IsClosed (.tabs cs T e)
 | cabs : CaptureSet.IsClosed cs -> CaptureBound.IsClosed cb -> Exp.IsClosed e ->
     Exp.IsClosed (.cabs cs cb e)
-| boxed : CaptureSet.IsClosed cs -> SepCtx.IsClosed Ψ -> Exp.IsClosed e ->
-    Exp.IsClosed (.boxed cs Ψ e)
 | reader : Var.IsClosed x -> Exp.IsClosed (.reader x)
 | pack : CaptureSet.IsClosed cs -> Var.IsClosed x -> Exp.IsClosed (.pack cs x)
 | app : Var.IsClosed x -> Var.IsClosed y -> Exp.IsClosed (.app x y)
 | tapp : Var.IsClosed x -> PureTy.IsClosed T -> Exp.IsClosed (.tapp x T)
 | capp : Var.IsClosed x -> CaptureSet.IsClosed cs -> Exp.IsClosed (.capp x cs)
-| unwrap : Var.IsClosed x -> Exp.IsClosed (.unwrap x)
 | letin : Exp.IsClosed e1 -> Exp.IsClosed e2 -> Exp.IsClosed (.letin e1 e2)
 | unpack : Exp.IsClosed e1 -> Exp.IsClosed e2 -> Exp.IsClosed (.unpack e1 e2)
 | unit : Exp.IsClosed .unit
