Semantic/Consume/Syntax.lean
@@ -1,7 +1,6 @@
 import Semantic.Consume.Syntax.Ty
 import Semantic.Consume.Syntax.Exp
 import Semantic.Consume.Syntax.Context
-import Semantic.Consume.Syntax.SepCtx
 
 /-!
 Syntax definitions for CC.
